Class: [[CSE 16]]
Subject: #computer-science #discrete-math 
Date: 2024-11-06
Teacher: **Prof. Musacchio**

# Direct Proof

## Introduction
- Sometimes we have to look at multiple cases before we can prove a statement is true

### Example 1
- *Proposition*: If $n \in \mathbb{N}$, then $1 + (−1)^n(2n − 1)$ is a multiple of $4$.
	- *Proof* Suppose $n \in \mathbb{N}$(Then $n$ is either even or odd.)
	- *Case 1*
		- *Suppose* $n$ is even.
		- *Then* $n = 2k$ for some $k \in \mathbb{Z}$, and $(−1)n = 1$.
		- *Thus* $1 + (−1)n(2n − 1) = 1 + (1)(2 · 2k − 1) = 4k$, which is a multiple of $4$.
	- *Case 2*
		- *Suppose* n is odd. 
		- Then $n = 2k + 1$ for some $k \in \mathbb{Z}$, and $(−1)n = −1$. 
		- Thus $1 + (−1)n(2n − 1) = 1 − (2(2k + 1) − 1) = −4k$, which is a multiple of $4$.